NLustre/Stream.v
@@ -39,34 +39,141 @@ if the clocked stream is [absent] at the corresponding instant. *)
   (** ** Synchronous functions *)
 
   (* With auxiliary hold function. *)
-  Fixpoint hold (r: stream bool) (v0: val) (xs: stream value) (n: nat) : val :=
+  (* Fixpoint hold (r: stream bool) (v0: val) (xs: stream value) (n: nat) : val := *)
+  (*   match n with *)
+  (*   | 0 => v0 *)
+  (*   | S m => *)
+  (*       match xs m with *)
+  (*       | absent => *)
+  (*         if r m then v0 else hold r v0 xs m *)
+  (*       | present hv => hv *)
+  (*       end *)
+  (*   end. *)
+
+  (* Definition fby (r: stream bool) (v0: val) (xs: stream value) : stream value := *)
+  (*   fun n => *)
+  (*     match xs n with *)
+  (*     | absent => absent *)
+  (*     | _ => present (if r n then v0 else hold r v0 xs n) *)
+  (*     end. *)
+
+  (* Definition mfby (r: stream bool) (xs: stream value) (ms: stream val) (ys: stream value) : Prop := *)
+  (*   forall n, *)
+  (*     match xs n with *)
+  (*     | absent => *)
+  (*       ms (S n) = (if r n then ms 0 else ms n) *)
+  (*       /\ ys n = absent *)
+  (*     | present v => *)
+  (*       ms (S n) = v *)
+  (*       /\ ys n = present (if r n then ms 0 else ms n) *)
+  (*     end. *)
+  Fixpoint hold (v0: val) (xs: stream value) (n: nat) : val :=
     match n with
     | 0 => v0
-    | S m =>
-        match xs m with
-        | absent =>
-          if r m then v0 else hold r v0 xs m
-        | present hv => hv
-        end
+    | S m => match xs m with
+            | absent => hold v0 xs m
+            | present hv => hv
+            end
     end.
 
-  Definition fby (r: stream bool) (v0: val) (xs: stream value) : stream value :=
+  Definition fby (v0: val) (xs: stream value) : stream value :=
     fun n =>
       match xs n with
       | absent => absent
-      | _ => present (if r n then v0 else hold r v0 xs n)
+      | _ => present (hold v0 xs n)
       end.
 
-  Definition mfby (r: stream bool) (xs: stream value) (ms: stream val) (ys: stream value) : Prop :=
-    forall n,
-      match xs n with
-      | absent =>
-        ms (S n) = (if r n then ms 0 else ms n)
-        /\ ys n = absent
-      | present v =>
-        ms (S n) = v
-        /\ ys n = present (if r n then ms 0 else ms n)
+  Require Import Coq.Arith.EqNat.
+  Require Import List.
+  Import List.ListNotations.
+  Open Scope list_scope.
+
+  Fixpoint take {A} (n: nat) (s: stream A) : list A :=
+    match n with
+    | O => nil
+    | S m => take m s ++ [s m]
+    end.
+
+  Fixpoint count (rs: cstream) (n: nat) : nat :=
+    match n, rs n with
+    | 0, false => 0
+    | 0, true => 1
+    | S m, false => count rs m
+    | S m, true => 1 + count rs m
+    end.
+
+  Definition mask {A} (opaque: A) (k: nat) (rs: cstream) (xs: stream A) : stream A :=
+    fun n =>
+      let c := count rs in
+      if beq_nat k (c n) then xs n else opaque.
+
+  (* Definition  *)
+  Definition mask_vs := @mask (list value) [].
+  Definition mask_v := mask absent.
+  Definition mask_b := mask false.
+
+  Definition r :=
+    fun n =>
+      match n with
+      | 0 => false
+      | 1 => false
+      | 2 => false
+      | 3 => true
+      | 4 => false
+      | 5 => false
+      | 6 => false
+      | 7 => false
+      | 8 => false
+      | 9 => true
+      | 10 => false
+      | 11 => false
+      | 12 => false
+      | 13 => true
+      | n => false
       end.
+
+  Notation "⊥" := (absent) (at level 50).
+  Notation "⇑" := (present true_val).
+  Notation "⇓" := (present false_val).
+  Notation "↑" := (true).
+  Notation "↓" := (false).
+
+  Fixpoint x n :=
+    match n with
+    | 0 => ⇓
+    | 1 => ⇑
+    | S (S n) => x n
+    end.
+
+  Compute (take 16 r, take 16 x, take 16 (count r),
+           take 16 (mask_v 0 r x),
+           take 16 (mask_v 1 r x),
+           take 16 (mask_v 2 r x),
+           take 16 (mask_v 3 r x),
+           take 16 (mask_v 4 r x)
+          ).
+
+  (* Remark mask_const_opaque: *)
+  (*   forall {A} n rs (opaque: A), *)
+  (*     mask opaque n rs (Streams.const opaque) ≡ Streams.const opaque. *)
+  (* Proof. *)
+  (*   cofix Cofix; intros. *)
+  (*   unfold_Stv rs; rewrite (unfold_Stream (Streams.const opaque)); *)
+  (*     constructor; destruct n as [|[]]; simpl; auto; try apply Cofix. *)
+  (*   reflexivity. *)
+  (* Qed. *)
+
+  (* CoFixpoint flatten_masks (bs: Stream bool) (xss: Stream (Stream value)) : Stream value := *)
+  (*   let xss := if hd bs then tl xss else xss in *)
+  (*   hd (hd xss) ::: flatten_masks (tl bs) (map (@tl value) xss). *)
+
+  (* CoFixpoint masks_from (n: nat) (rs: Stream bool) (xs: Stream value) : Stream (Stream value) := *)
+  (*   mask_v n rs xs ::: masks_from (n + 1) rs xs. *)
+
+  (* Definition masks := masks_from 0. *)
+
+  (* Eval simpl in take 16 (flatten_masks r (masks r x)). *)
+
   (** ** Properties *)
 
   Lemma present_injection:
